@prefix :     <https://mustrd.com/model/> .
@prefix dc:   <http://purl.org/dc/elements/1.1/> .
@prefix owl:  <http://www.w3.org/2002/07/owl#> .
@prefix rdf:  <http://www.w3.org/1999/02/22-rdf-syntax-ns#> .
@prefix xml:  <http://www.w3.org/XML/1998/namespace> .
@prefix xsd:  <http://www.w3.org/2001/XMLSchema#> .
@prefix foaf: <http://xmlns.com/foaf/spec/> .
@prefix rdfs: <http://www.w3.org/2000/01/rdf-schema#> .
@prefix skos: <http://www.w3.org/2004/02/skos/core#> .
@base <https://mustrd.com/model/> .

<https://mustrd.com/model>
    rdf:type owl:Ontology .

#################################################################
#    Object Properties
#################################################################

:dataset
    rdf:type         owl:ObjectProperty ;
    rdfs:domain      [ rdf:type    owl:Class ;
                       owl:unionOf ( :Compositedataset
                                     :Datasetexpectation
                                     :Given
                                     :Then ) ] ;
    rdfs:range       :Dataset ;
    rdfs:isDefinedBy <https://mustrd.com/model/> ;
    rdfs:label       "dataset" .


:expect
    rdf:type         owl:ObjectProperty ;
    rdfs:domain      :Then ;
    rdfs:range       :Expectation ;
    rdfs:isDefinedBy <https://mustrd.com/model/> ;
    rdfs:label       "expect" .


:given
    rdf:type         owl:ObjectProperty ;
    rdfs:domain      :TestSpec ;
    rdfs:range       :Given ;
    rdfs:isDefinedBy <https://mustrd.com/model/> ;
    rdfs:label       "given" .


:graph
    rdf:type         owl:ObjectProperty ;
    rdfs:domain      :Graphdataset ;
    rdfs:range       :Graph ;
    rdfs:isDefinedBy <https://mustrd.com/model/> ;
    rdfs:label       "graph" .


:hasspecs
    rdf:type         owl:ObjectProperty ;
    rdfs:domain      :TestSuite ;
    rdfs:range       :TestSpec ;
    rdfs:isDefinedBy <https://mustrd.com/model/> ;
    rdfs:label       "hasSpecs" .


:label_link-6c3eeabf-5c6d-4ea6-b61e-144df1e6a223
    rdf:type         owl:ObjectProperty ;
    rdfs:domain      :When ;
    rdfs:range       :Sparqlaction ;
    rdfs:isDefinedBy <https://mustrd.com/model/> ;
    rdfs:label       "label" .


:sparqlsource
    rdf:type         owl:ObjectProperty ;
    rdfs:domain      :Sparqlaction ;
    rdfs:range       :Sparqlsource ;
    rdfs:isDefinedBy <https://mustrd.com/model/> ;
    rdfs:label       "sparqlSource" .


:then
    rdf:type         owl:ObjectProperty ;
    rdfs:domain      :TestSpec ;
    rdfs:range       :Then ;
    rdfs:isDefinedBy <https://mustrd.com/model/> ;
    rdfs:label       "then" .


:when
    rdf:type         owl:ObjectProperty ;
    rdfs:domain      :TestSpec ;
    rdfs:range       :When ;
    rdfs:isDefinedBy <https://mustrd.com/model/> ;
    rdfs:label       "when" .


#################################################################
#    Data properties
#################################################################

:fileurl
    rdf:type         owl:DatatypeProperty ;
    rdfs:domain      :Filesparqlsource ;
    rdfs:comment     "a full or relatively qualified file:// url. Relative to what? We haven't thought that through, yet." ;
    rdfs:isDefinedBy <https://mustrd.com/model/> ;
    rdfs:label       "fileUrl" .


:flattendatasettotargetgraph
    rdf:type         owl:DatatypeProperty ;
    rdfs:domain      :Given ;
    rdfs:isDefinedBy <https://mustrd.com/model/> ;
    rdfs:label       "flattenDataSetToTargetGraph" .


:shouldflattengraph
    rdf:type         owl:DatatypeProperty ;
    rdfs:domain      :Graphdataset ;
    rdfs:isDefinedBy <https://mustrd.com/model/> ;
    rdfs:label       "shouldFlattenGraph" .


:sparql
    rdf:type         owl:DatatypeProperty ;
    rdfs:domain      :Sparqlaction ;
    rdfs:isDefinedBy <https://mustrd.com/model/> ;
    rdfs:label       "sparql" .


:targetgraph
    rdf:type         owl:DatatypeProperty ;
    rdfs:domain      [ rdf:type    owl:Class ;
                       owl:unionOf ( :Graphdataset
                                     :TestSpec ) ] ;
    rdfs:comment     "optional iri of a target graph to flatten into" ;
    rdfs:isDefinedBy <https://mustrd.com/model/> ;
    rdfs:label       "targetGraph" .


#################################################################
#    Classes
#################################################################

:Compositedataset
    rdf:type         owl:Class ;
    rdfs:subClassOf  :Dataset ;
    rdfs:isDefinedBy <https://mustrd.com/model/> ;
    rdfs:label       "CompositeDataSet" .


:ConstructSparql
    rdf:type         owl:Class ;
    rdfs:subClassOf  :Sparqlaction ;
    rdfs:isDefinedBy <https://mustrd.com/model/> ;
    rdfs:label       "ConstructSparql" .


:Dataset
    rdf:type         owl:Class ;
    rdfs:comment     "Some source of triples for comparison in either a Given or When clause" ;
    rdfs:isDefinedBy <https://mustrd.com/model/> ;
    rdfs:label       "DataSet" .


:Datasetexpectation
    rdf:type         owl:Class ;
    rdfs:subClassOf  :Expectation ;
    rdfs:comment     "A static dataset expectation. All DataSet(s) described by dataset will be composed into a single DataSet" ;
    rdfs:isDefinedBy <https://mustrd.com/model/> ;
    rdfs:label       "DatasetExpectation" .


:Expectation
    rdf:type         owl:Class ;
    rdfs:comment     """The expected result of the action performed in When, on the DataSet constructed, or composed in the Given. Expectations may be complete static datasets, results of ASKs, or a CONSTRUCT or SELECT and expected DataSet""" ;
    rdfs:isDefinedBy <https://mustrd.com/model/> ;
    rdfs:label       "Expectation" .


:Filesparqlsource
    rdf:type         owl:Class ;
    rdfs:subClassOf  :Sparqlsource ;
    rdfs:isDefinedBy <https://mustrd.com/model/> ;
    rdfs:label       "FileSparqlSource" .


:Given
    rdf:type         owl:Class ;
    rdfs:subClassOf  :Testspecsection ;
    rdfs:comment     "references one or more DataSet(s) to construct a precondition for this TestSpec" ;
    rdfs:isDefinedBy <https://mustrd.com/model/> ;
    rdfs:label       "Given" .


:Graph
    rdf:type         owl:Class ;
    rdfs:isDefinedBy <https://mustrd.com/model/> ;
    rdfs:label       "Graph" .


:Graphdataset
    rdf:type         owl:Class ;
    rdfs:subClassOf  :Dataset ;
    rdfs:isDefinedBy <https://mustrd.com/model/> ;
    rdfs:label       "GraphDataset" .


:Insertdeletesparql
    rdf:type         owl:Class ;
    rdfs:subClassOf  :Sparqlaction ;
    rdfs:isDefinedBy <https://mustrd.com/model/> ;
    rdfs:label       "InsertDeleteSparql" .


:S3sparqlsource
    rdf:type         owl:Class ;
    rdfs:subClassOf  :Sparqlsource ;
    rdfs:isDefinedBy <https://mustrd.com/model/> ;
    rdfs:label       "S3SparqlSource" .


:SelectSparql
    rdf:type         owl:Class ;
    rdfs:subClassOf  :Sparqlaction ;
    rdfs:isDefinedBy <https://mustrd.com/model/> ;
    rdfs:label       "SelectSparql" .


:Sparqlaction
    rdf:type         owl:Class ;
    rdfs:comment     "The sparql that is under-test. Either provided directly in the sparql property, or loaded courtesy a Sparql Loader from a disk source, db source, s3 source, etc." ;
    rdfs:isDefinedBy <https://mustrd.com/model/> ;
    rdfs:label       "SparqlAction" .


:Sparqlsource
    rdf:type         owl:Class ;
    rdfs:comment     """A source for the SPARQL action we want to execute in the When of a TestSpec.""" ;
    rdfs:isDefinedBy <https://mustrd.com/model/> ;
    rdfs:label       "SparqlSource" .


:StatementsDataset
    rdf:type         owl:Class ;
    rdfs:subClassOf  :Dataset ;
    rdfs:comment     "has a set of rdf:Statement(s) which will be unrotated/unreified back into the testing graph" ;
    rdfs:isDefinedBy <https://mustrd.com/model/> ;
    rdfs:label       "StatementsDataset" .


:TestSuite
    rdf:type         owl:Class ;
    rdfs:isDefinedBy <https://mustrd.com/model/> ;
    rdfs:label       "Test Suite" .


:TestSpec
    rdf:type         owl:Class ;
    rdfs:isDefinedBy <https://mustrd.com/model/> ;
    rdfs:label       "TestSpec" .


:Testspecsection
    rdf:type         owl:Class ;
    rdfs:isDefinedBy <https://mustrd.com/model/> ;
    rdfs:label       "TestSpecSection" .


:Then
    rdf:type         owl:Class ;
    rdfs:subClassOf  :Testspecsection ;
    rdfs:comment     """Describes the Expectation(s) of this part of a test.""" ;
    rdfs:isDefinedBy <https://mustrd.com/model/> ;
    rdfs:label       "Then" .


:When
    rdf:type         owl:Class ;
    rdfs:subClassOf  :Testspecsection ;
    rdfs:isDefinedBy <https://mustrd.com/model/> ;
    rdfs:label       "When" .


#################################################################
#    Individuals
#################################################################

:Emptydataset
    rdf:type         owl:NamedIndividual, :Dataset ;
    rdfs:comment     "So we can explicitly refer to a blank slate, empty dataset" ;
    rdfs:isDefinedBy <https://mustrd.com/model/> ;
    rdfs:label       "EmptyDataSet" .


#################################################################
#    Annotations
#################################################################

<https://mustrd.com/model>
    rdfs:comment "" ;
    rdfs:label   "Mustrd" .


###  Generated by the OWL API (version 5.1.17) https://github.com/owlcs/owlapi/
