@prefix :     <https://mustrd.com/model/> .
@prefix dc:   <http://purl.org/dc/elements/1.1/> .
@prefix gf:   <https://mustrd.com/model/> .
@prefix owl:  <http://www.w3.org/2002/07/owl#> .
@prefix rdf:  <http://www.w3.org/1999/02/22-rdf-syntax-ns#> .
@prefix xml:  <http://www.w3.org/XML/1998/namespace> .
@prefix xsd:  <http://www.w3.org/2001/XMLSchema#> .
@prefix foaf: <http://xmlns.com/foaf/spec/> .
@prefix rdfs: <http://www.w3.org/2000/01/rdf-schema#> .
@prefix skos: <http://www.w3.org/2004/02/skos/core#> .
@base <https://mustrd.com/model/> .

<https://mustrd.com/model>
    rdf:type owl:Ontology .

#################################################################
#    Object Properties
#################################################################

gf:dataset
    rdf:type         owl:ObjectProperty ;
    rdfs:domain      [ rdf:type    owl:Class ;
                       owl:unionOf ( gf:Compositedataset
                                     gf:Datasetexpectation
                                     gf:Given
                                     gf:Then ) ] ;
    rdfs:range       gf:Dataset ;
    rdfs:isDefinedBy <https://mustrd.com/model/> ;
    rdfs:label       "dataset" .


gf:expect
    rdf:type         owl:ObjectProperty ;
    rdfs:domain      gf:Then ;
    rdfs:range       gf:Expectation ;
    rdfs:isDefinedBy <https://mustrd.com/model/> ;
    rdfs:label       "expect" .


gf:given
    rdf:type         owl:ObjectProperty ;
    rdfs:domain      gf:TestSpec ;
    rdfs:range       gf:Given ;
    rdfs:isDefinedBy <https://mustrd.com/model/> ;
    rdfs:label       "given" .


gf:graph
    rdf:type         owl:ObjectProperty ;
    rdfs:domain      gf:Graphdataset ;
    rdfs:range       gf:Graph ;
    rdfs:isDefinedBy <https://mustrd.com/model/> ;
    rdfs:label       "graph" .


gf:hasspecs
    rdf:type         owl:ObjectProperty ;
    rdfs:domain      gf:TestSuite ;
    rdfs:range       gf:TestSpec ;
    rdfs:isDefinedBy <https://mustrd.com/model/> ;
    rdfs:label       "hasSpecs" .


gf:label_link-6c3eeabf-5c6d-4ea6-b61e-144df1e6a223
    rdf:type         owl:ObjectProperty ;
    rdfs:domain      gf:When ;
    rdfs:range       gf:Sparqlaction ;
    rdfs:isDefinedBy <https://mustrd.com/model/> ;
    rdfs:label       "label" .


gf:sparqlsource
    rdf:type         owl:ObjectProperty ;
    rdfs:domain      gf:Sparqlaction ;
    rdfs:range       gf:Sparqlsource ;
    rdfs:isDefinedBy <https://mustrd.com/model/> ;
    rdfs:label       "sparqlSource" .


gf:then
    rdf:type         owl:ObjectProperty ;
    rdfs:domain      gf:TestSpec ;
    rdfs:range       gf:Then ;
    rdfs:isDefinedBy <https://mustrd.com/model/> ;
    rdfs:label       "then" .


gf:when
    rdf:type         owl:ObjectProperty ;
    rdfs:domain      gf:TestSpec ;
    rdfs:range       gf:When ;
    rdfs:isDefinedBy <https://mustrd.com/model/> ;
    rdfs:label       "when" .


#################################################################
#    Data properties
#################################################################

gf:fileurl
    rdf:type         owl:DatatypeProperty ;
    rdfs:domain      gf:Filesparqlsource ;
    rdfs:comment     "a full or relatively qualified file:// url. Relative to what? We haven't thought that through, yet." ;
    rdfs:isDefinedBy <https://mustrd.com/model/> ;
    rdfs:label       "fileUrl" .


gf:flattendatasettotargetgraph
    rdf:type         owl:DatatypeProperty ;
    rdfs:domain      gf:Given ;
    rdfs:isDefinedBy <https://mustrd.com/model/> ;
    rdfs:label       "flattenDataSetToTargetGraph" .


gf:shouldflattengraph
    rdf:type         owl:DatatypeProperty ;
    rdfs:domain      gf:Graphdataset ;
    rdfs:isDefinedBy <https://mustrd.com/model/> ;
    rdfs:label       "shouldFlattenGraph" .


gf:sparql
    rdf:type         owl:DatatypeProperty ;
    rdfs:domain      gf:Sparqlaction ;
    rdfs:isDefinedBy <https://mustrd.com/model/> ;
    rdfs:label       "sparql" .


gf:targetgraph
    rdf:type         owl:DatatypeProperty ;
    rdfs:domain      [ rdf:type    owl:Class ;
                       owl:unionOf ( gf:Graphdataset
                                     gf:TestSpec ) ] ;
    rdfs:comment     "optional iri of a target graph to flatten into" ;
    rdfs:isDefinedBy <https://mustrd.com/model/> ;
    rdfs:label       "targetGraph" .


#################################################################
#    Classes
#################################################################

gf:Compositedataset
    rdf:type         owl:Class ;
    rdfs:subClassOf  gf:Dataset ;
    rdfs:isDefinedBy <https://mustrd.com/model/> ;
    rdfs:label       "CompositeDataSet" .


gf:ConstructSparql
    rdf:type         owl:Class ;
    rdfs:subClassOf  gf:Sparqlaction ;
    rdfs:isDefinedBy <https://mustrd.com/model/> ;
    rdfs:label       "ConstructSparql" .


gf:Dataset
    rdf:type         owl:Class ;
    rdfs:comment     "Some source of triples for comparison in either a Given or When clause" ;
    rdfs:isDefinedBy <https://mustrd.com/model/> ;
    rdfs:label       "DataSet" .


gf:Datasetexpectation
    rdf:type         owl:Class ;
    rdfs:subClassOf  gf:Expectation ;
    rdfs:comment     "A static dataset expectation. All DataSet(s) described by dataset will be composed into a single DataSet" ;
    rdfs:isDefinedBy <https://mustrd.com/model/> ;
    rdfs:label       "DatasetExpectation" .


gf:Expectation
    rdf:type         owl:Class ;
    rdfs:comment     """The expected result of the action performed in When, on the DataSet constructed, or composed in the Given. Expectations may be complete static datasets, results of ASKs, or a CONSTRUCT or SELECT and expected DataSet""" ;
    rdfs:isDefinedBy <https://mustrd.com/model/> ;
    rdfs:label       "Expectation" .


gf:Filesparqlsource
    rdf:type         owl:Class ;
    rdfs:subClassOf  gf:Sparqlsource ;
    rdfs:isDefinedBy <https://mustrd.com/model/> ;
    rdfs:label       "FileSparqlSource" .


gf:Given
    rdf:type         owl:Class ;
    rdfs:subClassOf  gf:Testspecsection ;
    rdfs:comment     "references one or more DataSet(s) to construct a precondition for this TestSpec" ;
    rdfs:isDefinedBy <https://mustrd.com/model/> ;
    rdfs:label       "Given" .


gf:Graph
    rdf:type         owl:Class ;
    rdfs:isDefinedBy <https://mustrd.com/model/> ;
    rdfs:label       "Graph" .


gf:Graphdataset
    rdf:type         owl:Class ;
    rdfs:subClassOf  gf:Dataset ;
    rdfs:isDefinedBy <https://mustrd.com/model/> ;
    rdfs:label       "GraphDataset" .


gf:Insertdeletesparql
    rdf:type         owl:Class ;
    rdfs:subClassOf  gf:Sparqlaction ;
    rdfs:isDefinedBy <https://mustrd.com/model/> ;
    rdfs:label       "InsertDeleteSparql" .


gf:S3sparqlsource
    rdf:type         owl:Class ;
    rdfs:subClassOf  gf:Sparqlsource ;
    rdfs:isDefinedBy <https://mustrd.com/model/> ;
    rdfs:label       "S3SparqlSource" .


gf:SelectSparql
    rdf:type         owl:Class ;
    rdfs:subClassOf  gf:Sparqlaction ;
    rdfs:isDefinedBy <https://mustrd.com/model/> ;
    rdfs:label       "SelectSparql" .


gf:Sparqlaction
    rdf:type         owl:Class ;
    rdfs:comment     "The sparql that is under-test. Either provided directly in the sparql property, or loaded courtesy a Sparql Loader from a disk source, db source, s3 source, etc." ;
    rdfs:isDefinedBy <https://mustrd.com/model/> ;
    rdfs:label       "SparqlAction" .


gf:Sparqlsource
    rdf:type         owl:Class ;
    rdfs:comment     """A source for the SPARQL action we want to execute in the When of a TestSpec.""" ;
    rdfs:isDefinedBy <https://mustrd.com/model/> ;
    rdfs:label       "SparqlSource" .


gf:Statementsdataset
    rdf:type         owl:Class ;
    rdfs:subClassOf  gf:Dataset ;
    rdfs:comment     "has a set of rdf:Statement(s) which will be unrotated/unreified back into the testing graph" ;
    rdfs:isDefinedBy <https://mustrd.com/model/> ;
    rdfs:label       "StatementsDataSet" .


gf:TestSuite
    rdf:type         owl:Class ;
    rdfs:isDefinedBy <https://mustrd.com/model/> ;
    rdfs:label       "Test Suite" .


gf:TestSpec
    rdf:type         owl:Class ;
    rdfs:isDefinedBy <https://mustrd.com/model/> ;
    rdfs:label       "TestSpec" .


gf:Testspecsection
    rdf:type         owl:Class ;
    rdfs:isDefinedBy <https://mustrd.com/model/> ;
    rdfs:label       "TestSpecSection" .


gf:Then
    rdf:type         owl:Class ;
    rdfs:subClassOf  gf:Testspecsection ;
    rdfs:comment     """Describes the Expectation(s) of this part of a test.""" ;
    rdfs:isDefinedBy <https://mustrd.com/model/> ;
    rdfs:label       "Then" .


gf:When
    rdf:type         owl:Class ;
    rdfs:subClassOf  gf:Testspecsection ;
    rdfs:isDefinedBy <https://mustrd.com/model/> ;
    rdfs:label       "When" .


#################################################################
#    Individuals
#################################################################

gf:Emptydataset
    rdf:type         owl:NamedIndividual, gf:Dataset ;
    rdfs:comment     "So we can explicitly refer to a blank slate, empty dataset" ;
    rdfs:isDefinedBy <https://mustrd.com/model/> ;
    rdfs:label       "EmptyDataSet" .


#################################################################
#    Annotations
#################################################################

<https://mustrd.com/model>
    rdfs:comment "" ;
    rdfs:label   "Mustrd" .


###  Generated by the OWL API (version 5.1.17) https://github.com/owlcs/owlapi/
